Fix code extractions for abstract bplustrees

BPlusTree_Set.thy
@@ -146,15 +146,6 @@ lemma isin_sorted: "sorted_less (xs@a#ys) \<Longrightarrow>
 
 (* lift to split *)
 
-lemma leaves_conc: "leaves (Node (ls@rs) t) = leaves_list ls @ leaves_list rs @ leaves t"
-  apply(induction ls)
-  apply auto
-  done
-
-lemma leaves_split: "split ts x = (ls,rs) \<Longrightarrow> leaves (Node ts t) = leaves_list ls @ leaves_list rs @ leaves t"
-  using leaves_conc split_conc by blast
-
-
 
 lemma isin_sorted_split:
   assumes "Laligned (Node ts t) u"
@@ -176,7 +167,7 @@ next
     using assms sorted_cons sorted_snoc 
     by blast
   moreover have leaves_split: "leaves (Node ts t) = leaves_list ls @ leaves_list rs @ leaves t"
-    using assms(3) leaves_split by blast
+    using assms(3) split_tree.leaves_split by blast
   then show ?thesis
   proof (cases "leaves_list ls")
     case Nil
@@ -1023,7 +1014,7 @@ next
     using assms ls_tail_split
     by auto
   moreover have leaves_split: "leaves (Node ts t) = leaves_list ls @ leaves_list rs @ leaves t"
-    using assms(3) leaves_split by blast
+    using assms(3) split_tree.leaves_split by blast
   then show ?thesis
   proof (cases "leaves_list ls")
     case Nil
@@ -1088,7 +1079,7 @@ proof -
     moreover have "sorted_less (leaves sub @ [r'])"
     proof -
       have "sorted_less (leaves_list ls @ leaves sub @ leaves_list rs @ leaves t)"
-        using assms(1) assms(2) split_set.leaves_split split_set_axioms by fastforce
+        using assms(1) assms(2) split_tree.leaves_split split_set_axioms by fastforce
       then show ?thesis
         using assms 
         by (metis Cons sorted_mid_iff sorted_wrt_append)
@@ -2932,7 +2923,7 @@ next
     using assms ls_tail_split sorted_inorder sorted_inorder_separators
     by blast
   moreover have leaves_split: "leaves (Node ts t) = leaves_list ls @ leaves_list rs @ leaves t"
-    using assms(3) leaves_split by blast
+    using assms(3) split_tree.leaves_split by blast
   then show ?thesis
   proof (cases "leaves_list ls")
     case Nil
@@ -3670,115 +3661,6 @@ sublocale split_set split isin_list insert_list delete_list
   by unfold_locales auto
 
 end
-
-global_interpretation bplustree_linear_search:
-    split_set linear_split bplustree_ls_isin_list bplustree_ls_insert_list bplustree_ls_delete_list
-  (* the below definitions are required to be set here for evaluating example code... *)
-  defines bplustree_ls_isin = bplustree_linear_search.isin 
-    and bplustree_ls_ins = bplustree_linear_search.ins
-    and bplustree_ls_insert = bplustree_linear_search.insert
-    and bplustree_ls_del = bplustree_linear_search.del
-    and bplustree_ls_delete = bplustree_linear_search.delete
-  apply unfold_locales
-  unfolding linear_split.simps
-  subgoal by (auto split: list.splits)
-  subgoal
-    apply (auto split: list.splits)
-    by (metis (no_types, lifting) case_prodD in_set_conv_decomp takeWhile_eq_all_conv takeWhile_idem)
-  subgoal by (metis case_prod_conv hd_dropWhile le_less_linear list.sel(1) list.simps(3))
-  subgoal using bplustree_linear_search_list.isin_list_set by blast
-  subgoal using bplustree_linear_search_list.insert_list_set by blast
-  subgoal using bplustree_linear_search_list.delete_list_set by blast
-  done
-
-
-text "Some examples follow to show that the implementation works
-      and the above lemmas make sense. The examples are visualized in the thesis."
-
-abbreviation "bplustree\<^sub>q \<equiv> bplustree_ls_isin"
-abbreviation "bplustree\<^sub>i \<equiv> bplustree_ls_insert"
-abbreviation "bplustree\<^sub>d \<equiv> bplustree_ls_delete"
-
-definition "uint8_max \<equiv> 2^8-1::nat"
-declare uint8_max_def[simp]
-
-typedef uint8 = "{n::nat. n \<le> uint8_max}" 
-  by auto
-
-setup_lifting type_definition_uint8
-
-instantiation uint8 :: linorder
-begin
-
-lift_definition less_eq_uint8 :: "uint8 \<Rightarrow> uint8 \<Rightarrow> bool"
-  is "(less_eq::nat \<Rightarrow> nat \<Rightarrow> bool)" .
-
-lift_definition less_uint8 :: "uint8 \<Rightarrow> uint8 \<Rightarrow> bool"
-  is "(less::nat \<Rightarrow> nat \<Rightarrow> bool)" .
-
-instance
-  by standard (transfer; auto)+
-end
-
-instantiation uint8 :: order_top
-begin
-
-lift_definition top_uint8 :: uint8 is "uint8_max::nat"
-  by simp
-
-
-instance 
-  by standard (transfer; simp)
-end
-
-
-instantiation uint8 :: numeral
-begin
-
-lift_definition one_uint8 :: uint8 is "1::nat"
-  by auto
-
-lift_definition plus_uint8 :: "uint8 \<Rightarrow> uint8 \<Rightarrow> uint8"
-  is "\<lambda>a b. min (a + b) uint8_max"
-  by simp
-
-instance by standard (transfer; auto)
-end
-
-instantiation uint8 :: equal
-begin
-
-lift_definition equal_uint8 :: "uint8 \<Rightarrow> uint8 \<Rightarrow> bool"
-  is "(=)" .
-
-instance by standard (transfer; auto)
-end
-
-
-value "uint8_max"
-
-value "let k=2::nat; x::uint8 bplustree = (Node [(Node [(LNode [1,2], 2),(LNode [3,4], 4),(LNode [5,6,7], 8)] (LNode [9,10]), 10)] (Node [(LNode [11,12,13,14], 14), (LNode [15,17], 20)] (LNode [21,22,23]))) in
-      root_order k x"
-value "let k=2::nat; x::uint8 bplustree = (Node [(Node [(LNode [1,2], 2),(LNode [3,4], 4),(LNode [5,6,7], 8)] (LNode [9,10]), 10)] (Node [(LNode [11,12,13,14], 14), (LNode [15,17], 20)] (LNode [21,22,23]))) in
-      bal x"
-value "let k=2::nat; x::uint8 bplustree = (Node [(Node [(LNode [1,2], 2),(LNode [3,4], 4),(LNode [5,6,7], 8)] (LNode [9,10]), 10)] (Node [(LNode [11,12,13,14], 14), (LNode [15,17], 20)] (LNode [50,55,56]))) in
-      sorted_less (leaves x)"
-value "let k=2::nat; x::uint8 bplustree = (Node [(Node [(LNode [1,2], 2),(LNode [3,4], 4),(LNode [5,6,7], 8)] (LNode [9,10]), 10)] (Node [(LNode [11,12,13,14], 14), (LNode [15,17], 20)] (LNode [50,55,56]))) in
-      Laligned x top"
-value "let k=2::nat; x::uint8 bplustree = (Node [(Node [(LNode [1,2], 2),(LNode [3,4], 4),(LNode [5,6,7], 8)] (LNode [9,10]), 10)] (Node [(LNode [11,12,13,14], 14), (LNode [15,17], 20)] (LNode [50,55,56]))) in
-      x"
-value "let k=2::nat; x::uint8 bplustree = (Node [(Node [(LNode [1,2], 2),(LNode [3,4], 4),(LNode [5,6,7], 8)] (LNode [9,10]), 10)] (Node [(LNode [11,12,13,14], 14), (LNode [15,17], 20)] (LNode [50,55,56]))) in
-      bplustree\<^sub>q x 4"
-value "let k=2::nat; x::uint8 bplustree = (Node [(Node [(LNode [1,2], 2),(LNode [3,4], 4),(LNode [5,6,7], 8)] (LNode [9,10]), 10)] (Node [(LNode [11,12,13,14], 14), (LNode [15,17], 20)] (LNode [50,55,56]))) in
-      bplustree\<^sub>q x 20"
-value "let k=2::nat; x::uint8 bplustree = (Node [(Node [(LNode [1,2], 2),(LNode [3,4], 4),(LNode [5,6,7], 8)] (LNode [9,10]), 10)] (Node [(LNode [11,12,13,14], 14), (LNode [15,17], 20)] (LNode [50,55,56]))) in
-      bplustree\<^sub>i k 9 x"
-value "let k=2::nat; x::uint8 bplustree = (Node [(Node [(LNode [1,2], 2),(LNode [3,4], 4),(LNode [5,6,7], 8)] (LNode [9,10]), 10)] (Node [(LNode [11,12,13,14], 14), (LNode [15,17], 20)] (LNode [50,55,56]))) in
-      bplustree\<^sub>i k 1 (bplustree\<^sub>i k 9 x)"
-value "let k=2::nat; x::uint8 bplustree = (Node [(Node [(LNode [1,2], 2),(LNode [3,4], 4),(LNode [5,6,7], 8)] (LNode [9,10]), 10)] (Node [(LNode [11,12,13,14], 14), (LNode [15,17], 20)] (LNode [50,55,56]))) in
-      bplustree\<^sub>d k 10 (bplustree\<^sub>i k 1 (bplustree\<^sub>i k 9 x))"
-value "let k=2::nat; x::uint8 bplustree = (Node [(Node [(LNode [1,2], 2),(LNode [3,4], 4),(LNode [5,6,7], 8)] (LNode [9,10]), 10)] (Node [(LNode [11,12,13,14], 14), (LNode [15,17], 20)] (LNode [50,55,56]))) in
-      bplustree\<^sub>d k 3 (bplustree\<^sub>d k 10 (bplustree\<^sub>i k 1 (bplustree\<^sub>i k 9 x)))"
 
 
 end
