BPlusTree_ImpSplitCE.thy
@@ -1,0 +1,107 @@
+theory BPlusTree_ImpSplitCE
+  imports
+    BPlusTree_ImpRange
+    BPlusTree_ImpSet
+begin
+
+
+subsection "Obtaining executable code"
+
+text "In order to obtain fully defined functions,
+we need to plug our split function implementations
+into the locales we introduced previously."
+
+global_interpretation bplustree_imp_binary_split_list_lrange: imp_split_list_smeq bin'_split
+  defines bplustree_lrange_list = bplustree_imp_binary_split_list_lrange.imp_lrange_list
+  apply unfold_locales
+  by(sep_auto heap add: bin'_split_rule)
+
+
+global_interpretation bplustree_imp_binary_split_range: 
+  imp_split_range linear_split bplustree_linear_search_list.lrange_split bin_split bplustree_lrange_list
+  apply unfold_locales
+  subgoal by (simp add: bplustree_linear_search_list.lrange_split_req)
+  subgoal 
+    apply(simp add: bplustree_lrange_list_def)
+    apply(vcg heap: bplustree_imp_binary_split_list.imp_lrange_list_rule)
+  done
+
+find_theorems bplustree_lrange
+find_theorems bplustree_lrange_list
+find_theorems imp_split_range.concat_leafs_range
+find_theorems bplustree_leafs_range
+
+export_code bplustree_leafs_range bplustree_lrange checking OCaml SML Scala
+export_code bplustree_lrange in OCaml module_name BPlusTree
+export_code bplustree_lrange in SML module_name BPlusTree
+export_code bplustree_lrange in Scala module_name BPlusTree
+
+global_interpretation bplustree_imp_binary_split_list: imp_split_list_smeq bin'_split
+  defines bplustree_isin_list = bplustree_imp_binary_split_list.imp_isin_list
+    and bplustree_ins_list = bplustree_imp_binary_split_list.imp_ins_list
+    and bplustree_del_list = bplustree_imp_binary_split_list.imp_del_list
+  apply unfold_locales
+  apply(sep_auto heap: bin'_split_rule)
+  done
+
+print_theorems
+
+
+
+global_interpretation bplustree_imp_binary_split_set: 
+  imp_split_set bplustree_ls_isin_list bplustree_ls_insert_list bplustree_ls_delete_list
+  linear_split bin_split bplustree_isin_list bplustree_ins_list bplustree_del_list
+  defines bplustree_isin = bplustree_imp_binary_split_set.isin
+    and bplustree_ins = bplustree_imp_binary_split_set.ins
+    and bplustree_insert = bplustree_imp_binary_split_set.insert
+    (*and bplustree_del = bplustree_imp_binary_split.del
+    and bplustree_delete = bplustree_imp_binary_split.delete*)
+    and bplustree_empty = bplustree_imp_binary_split_set.empty
+  apply unfold_locales
+  subgoal
+    apply(vcg heap: bplustree_imp_binary_split_list.imp_isin_list_rule)
+    apply (simp add: bplustree_ls_isin_list_def)
+    done
+  subgoal
+    apply(vcg heap: bplustree_imp_binary_split_list.imp_ins_list_rule)
+    apply (simp add: bplustree_ls_insert_list_def)
+    done
+  subgoal
+    apply(vcg heap: bplustree_imp_binary_split_list.imp_del_list_rule)
+    apply (simp add: bplustree_ls_delete_list_def)
+    done
+  done
+
+declare bplustree_imp_binary_split_set.ins.simps[code]
+declare bplustree_imp_binary_split_set.isin.simps[code]
+
+export_code bplustree_empty bplustree_isin bplustree_insert checking OCaml SML Scala
+export_code bplustree_empty bplustree_isin bplustree_insert in OCaml module_name BPlusTree
+export_code bplustree_empty bplustree_isin bplustree_insert in SML module_name BPlusTree
+export_code bplustree_empty bplustree_isin bplustree_insert in Scala module_name BPlusTree
+
+
+
+interpretation bplustree_imp_linear_split_tree: imp_split_tree_smeq lin_split
+  apply unfold_locales
+  apply(sep_auto heap: lin_split_rule)
+  done
+
+
+text "Obtaining actual code turns out to be slightly more difficult
+  due to the use of locales. However, we successfully obtain
+the B-tree insertion and membership query with binary search splitting."
+
+(* interpretation bplustree_imp_binary_split_list: imp_split_list_smeq bin'_split
+  apply unfold_locales
+  apply(sep_auto heap: bin'_split_rule)
+  done
+*)
+
+interpretation bplustree_imp_bin_split_tree: imp_split_tree_smeq bin_split
+  apply unfold_locales
+  apply(sep_auto heap: bin_split_rule)
+  done
+
+
+end
