start_isabelle.sh
@@ -1,4 +1,4 @@
 #! /bin/bash
 
-isabelle components -u /usr/bin/Isabelle2021/afp-2021-10-19/thys
+isabelle components -u $HOME/bin/Isabelle2021/afp-2021-10-19/thys
 isabelle jedit -l Refine_Imperative_HOL
